add enterprise

deps/poulet4/lib/P4automata/Benchmarks/Enterprise.v
@@ -13,35 +13,367 @@ Require Import Coq.Program.Equality.
 
 Open Scope p4a.
 
-Notation eth_size := 112.
-Notation vlan_size := 160.
-Notation ipv4_size := 64.
-Notation ipv6_size := 64.
-Notation icmp_size := 32.
-Notation tcp_size := 160.
-Notation udp_size := 160.
-Notation arp_size := 64.
+Module Simple.
 
-Inductive header: nat -> Type :=
-| HdrEth: header eth_size
-| HdrVLAN0: header vlan_size
-| HdrVLAN1: header vlan_size
-| HdrIPv4: header ipv4_size
-| HdrIPv6: header ipv6_size
-| HdrTCP: header tcp_size
-| HdrUDP: header udp_size
-| HdrICMP: header icmp_size
-| HdrICMPv6: header icmp_size
-| HdrARP: header arp_size
-| HdrARPIP: header ipv4_size.
+  Notation eth_size := 112.
+  Notation vlan_size := 160.
+  Notation ipv4_size := 64.
+  Notation ipv6_size := 64.
+  Notation icmp_size := 32.
+  Notation tcp_size := 160.
+  Notation udp_size := 160.
+  Notation arp_size := 64.
 
-Derive Signature for header.
-Definition h112_eq_dec (x y: header 112) : {x = y} + {x <> y}.
+  Inductive header: nat -> Type :=
+  | HdrEth: header eth_size
+  | HdrVLAN0: header vlan_size
+  | HdrVLAN1: header vlan_size
+  | HdrIPv4: header ipv4_size
+  | HdrIPv6: header ipv6_size
+  | HdrTCP: header tcp_size
+  | HdrUDP: header udp_size
+  | HdrICMP: header icmp_size
+  | HdrICMPv6: header icmp_size
+  | HdrARP: header arp_size
+  | HdrARPIP: header ipv4_size.
+
+  Derive Signature for header.
+  Definition h112_eq_dec (x y: header 112) : {x = y} + {x <> y}.
+  refine (
+    match x with
+    | HdrEth =>
+      match y with
+      | HdrEth => left eq_refl
+      end
+    end
+  ); unfold "<>"; intros H; inversion H.
+  Defined.
+  Definition h32_eq_dec (x y: header 32) : {x = y} + {x <> y}.
+  refine (
+    match x with
+    | HdrICMP =>
+      match y with
+      | HdrICMP => left eq_refl
+      | HdrICMPv6 => right _
+      end
+    | HdrICMPv6 =>
+      match y with
+      | HdrICMP => right _
+      | HdrICMPv6 => left eq_refl
+      end
+    end
+  ); unfold "<>"; intros H; inversion H.
+  Defined.
+  Definition h64_eq_dec (x y: header 64) : {x = y} + {x <> y}.
+  refine (
+    match x with
+    | HdrIPv4 =>
+      match y with
+      | HdrIPv4 => left eq_refl
+      | HdrIPv6 => right _
+      | HdrARP => right _
+      | HdrARPIP => right _
+      end
+    | HdrIPv6 =>
+      match y with
+      | HdrIPv4 => right _
+      | HdrIPv6 => left eq_refl
+      | HdrARP => right _
+      | HdrARPIP => right _
+      end
+    | HdrARP =>
+      match y with
+      | HdrIPv4 => right _
+      | HdrIPv6 => right _
+      | HdrARP => left eq_refl
+      | HdrARPIP => right _
+      end
+    | HdrARPIP =>
+      match y with
+      | HdrIPv4 => right _
+      | HdrIPv6 => right _
+      | HdrARP => right _
+      | HdrARPIP => left eq_refl
+      end
+    end
+  ); unfold "<>"; intros H; inversion H.
+  Defined.
+  Definition h160_eq_dec (x y: header 160) : {x = y} + {x <> y}.
+  refine (
+    match x with
+    | HdrVLAN0 =>
+      match y with
+      | HdrVLAN0 => left eq_refl
+      | HdrVLAN1 => right _
+      | HdrTCP => right _
+      | HdrUDP => right _
+      end
+    | HdrVLAN1 =>
+      match y with
+      | HdrVLAN0 => right _
+      | HdrVLAN1 => left eq_refl
+      | HdrTCP => right _
+      | HdrUDP => right _
+      end
+    | HdrTCP =>
+      match y with
+      | HdrVLAN0 => right _
+      | HdrVLAN1 => right _
+      | HdrTCP => left eq_refl
+      | HdrUDP => right _
+      end
+    | HdrUDP =>
+      match y with
+      | HdrVLAN0 => right _
+      | HdrVLAN1 => right _
+      | HdrTCP => right _
+      | HdrUDP => left eq_refl
+      end
+    end
+  ); unfold "<>"; intros H; inversion H.
+  Defined.
+  Definition header_eqdec_ (n: nat) (x: header n) (y: header n) : {x = y} + {x <> y}.
+    solve_header_eqdec_ n x y
+      ((existT (fun n => forall x y: header n, {x = y} + {x <> y}) _ h112_eq_dec) ::
+      (existT _ _ h32_eq_dec) ::
+      (existT _ _ h64_eq_dec) ::
+      (existT _ _ h160_eq_dec) ::
+        nil).
+  Defined.
+
+  Global Instance header_eqdec: forall n, EquivDec.EqDec (header n) eq := header_eqdec_.
+  Global Instance header_eqdec': EquivDec.EqDec (Syntax.H' header) eq.
+    solve_eqdec'.
+  Defined.
+  Global Instance header_finite: forall n, @Finite (header n) _ _.
+    intros n; solve_indexed_finiteness n [112; 32 ; 64 ; 160 ].
+  Qed.
+
+  Global Program Instance header_finite': @Finite {n & header n} _ header_eqdec' :=
+    {| enum := [
+        existT _ _ HdrEth
+      ; existT _ _ HdrVLAN0
+      ; existT _ _ HdrVLAN1
+      ; existT _ _ HdrIPv4
+      ; existT _ _ HdrIPv6
+      ; existT _ _ HdrTCP
+      ; existT _ _ HdrUDP
+      ; existT _ _ HdrICMP
+      ; existT _ _ HdrICMPv6
+      ; existT _ _ HdrARP
+      ; existT _ _ HdrARPIP
+      ] |}.
+  Next Obligation.
+    solve_header_finite.
+  Qed.
+  Next Obligation.
+  dependent destruction X; subst;
+  repeat (
+    match goal with
+    | |- ?L \/ ?R => (now left; trivial) || right
+    end
+  ).
+  Qed.
+
+  Inductive state: Type :=
+  | ParseEth
+  | ParseVLAN0
+  | ParseVLAN1
+  | ParseIPv4
+  | ParseIPv6
+  | ParseTCP
+  | ParseUDP
+  | ParseICMP
+  | ParseICMPv6
+  | ParseARP
+  | ParseARPIP.
+
+  Scheme Equality for state.
+  Global Instance state_eqdec: EquivDec.EqDec state eq := state_eq_dec.
+  Global Program Instance state_finite: @Finite state _ state_eq_dec :=
+    {| enum := [ParseEth; ParseVLAN0; ParseVLAN1; ParseIPv4; ParseIPv6; ParseTCP; ParseUDP; ParseICMP; ParseICMPv6; ParseARP; ParseARPIP] |}.
+  Next Obligation.
+    repeat constructor;
+      repeat match goal with
+              | H: List.In _ [] |- _ => apply List.in_nil in H; exfalso; exact H
+              | |- ~ List.In _ [] => apply List.in_nil
+              | |- ~ List.In _ (_ :: _) => unfold not; intros
+              | H: List.In _ (_::_) |- _ => inversion H; clear H
+              | _ => discriminate
+              end.
+  Qed.
+  Next Obligation.
+    destruct x; intuition congruence.
+  Qed.
+
+  Definition states (s: state) : P4A.state state header :=
+    match s with
+    | ParseEth =>
+      {| st_op := extract(HdrEth);
+        st_trans := transition select (| (EHdr HdrEth)[111--96] |)
+                                {{ [| hexact 0x8100 |] ==> inl ParseVLAN0 ;;;
+                                  [| hexact 0x9100 |] ==> inl ParseVLAN0 ;;;
+                                  [| hexact 0x9200 |] ==> inl ParseVLAN0 ;;;
+                                  [| hexact 0x9300 |] ==> inl ParseVLAN0 ;;;
+                                  [| hexact 0x0800 |] ==> inl ParseIPv4 ;;;
+                                  [| hexact 0x86dd |] ==> inl ParseIPv6 ;;;
+                                  [| hexact 0x0806 |] ==> inl ParseARP ;;;
+                                  [| hexact 0x8035 |] ==> inl ParseARP ;;;
+                                  reject }}
+      |}
+    | ParseVLAN0 =>
+      {| st_op := extract(HdrVLAN0) ;
+        st_trans := transition select (| (EHdr HdrVLAN0)[159--144] |)
+                                {{ [| hexact 0x8100 |] ==> inl ParseVLAN1 ;;;
+                                  [| hexact 0x9100 |] ==> inl ParseVLAN1 ;;;
+                                  [| hexact 0x9200 |] ==> inl ParseVLAN1 ;;;
+                                  [| hexact 0x9300 |] ==> inl ParseVLAN1 ;;;
+                                  [| hexact 0x0800 |] ==> inl ParseIPv4 ;;;
+                                  [| hexact 0x86dd |] ==> inl ParseIPv6 ;;;
+                                  [| hexact 0x0806 |] ==> inl ParseARP ;;;
+                                  [| hexact 0x8035 |] ==> inl ParseARP ;;;
+                                  reject }}
+      |}
+    | ParseVLAN1 =>
+      {| st_op := extract(HdrVLAN1) ;
+        st_trans := transition select (| (EHdr HdrVLAN1)[159--144] |)
+                                {{ [| hexact 0x0800 |] ==> inl ParseIPv4 ;;;
+                                  [| hexact 0x86dd |] ==> inl ParseIPv6 ;;;
+                                  [| hexact 0x0806 |] ==> inl ParseARP ;;;
+                                  [| hexact 0x8035 |] ==> inl ParseARP ;;;
+                                  reject }}
+      |}
+    | ParseIPv4 =>
+      {| st_op := extract(HdrIPv4);
+        st_trans := transition select (| (EHdr HdrIPv4)[79--72] |)
+                                {{ [| hexact 1 |] ==> inl ParseICMP;;;
+                                  [| hexact 6 |] ==> inl ParseTCP;;;
+                                  [| hexact 17 |] ==> inl ParseUDP;;;
+                                  accept
+                                }}
+      |}
+    | ParseIPv6 =>
+      {| st_op := extract(HdrIPv6);
+        st_trans := transition select (| (EHdr HdrIPv6)[55--48] |)
+                                {{ [| hexact 1 |] ==> inl ParseICMPv6;;;
+                                  [| hexact 6 |] ==> inl ParseTCP;;;
+                                  [| hexact 17 |] ==> inl ParseUDP;;;
+                                  accept
+                                }}
+      |}
+    | ParseUDP =>
+      {| st_op := extract(HdrUDP);
+        st_trans := transition accept |}
+    | ParseTCP =>
+      {| st_op := extract(HdrTCP);
+        st_trans := transition accept |}
+    | ParseICMP =>
+      {| st_op := extract(HdrICMP);
+        st_trans := transition accept |}
+    | ParseICMPv6 =>
+      {| st_op := extract(HdrICMPv6);
+        st_trans := transition accept |}
+    | ParseARP =>
+      {| st_op := extract(HdrARP);
+        st_trans := transition select (| (EHdr HdrARP)[31--16] |)
+                                {{ [| hexact 0x0800 |] ==> inl ParseARPIP;;;
+                                  accept
+                                }}
+      |}
+    | ParseARPIP =>
+      {| st_op := extract(HdrARPIP);
+        st_trans := transition accept
+      |}
+    end.
+
+  Program Definition aut: Syntax.t state header :=
+    {| t_states := states |}.
+  Solve Obligations with (destruct s; cbv; Lia.lia).
+End Simple.
+(* 
+Module Optimized.
+Inductive state := | State_1_suff_12 | State_7_suff_3 | State_4_suff_0 | State_1 | State_0_suff_0 | State_2_suff_3 | State_6_suff_0 | State_7 | State_8 | State_9 | State_6_suff_3 | State_1_suff_11 | State_5_suff_2 | State_1_suff_7 | State_0 | State_8_suff_1 | State_4_suff_3 | State_3_suff_0 | State_2_suff_1 | State_5_suff_0 | State_9_suff_1 | State_4_suff_2 | State_8_suff_0 | State_5_suff_1 | State_9_suff_0 | State_7_suff_2 | State_2 | State_7_suff_0 | State_8_suff_3 | State_8_suff_2 | State_1_suff_10 | State_9_suff_3 | State_10_suff_1 | State_6_suff_1 | State_4_suff_1 | State_10 | State_3 | State_2_suff_0 | State_5 | State_6 | State_9_suff_2 | State_1_suff_6 | State_3_suff_1 | State_2_suff_2 | State_1_suff_3 | State_4 | State_6_suff_2 | State_9_suff_6 | State_1_suff_5 | State_7_suff_1 | State_10_suff_0 | State_5_suff_3.
+Scheme Equality for state.
+Global Instance state_eqdec: EquivDec.EqDec state eq := state_eq_dec.
+Global Program Instance state_finite: @Finite state _ state_eq_dec :=
+  {| enum := [State_1_suff_12; State_7_suff_3; State_4_suff_0; State_1; State_0_suff_0; State_2_suff_3; State_6_suff_0; State_7; State_8; State_9; State_6_suff_3; State_1_suff_11; State_5_suff_2; State_1_suff_7; State_0; State_8_suff_1; State_4_suff_3; State_3_suff_0; State_2_suff_1; State_5_suff_0; State_9_suff_1; State_4_suff_2; State_8_suff_0; State_5_suff_1; State_9_suff_0; State_7_suff_2; State_2; State_7_suff_0; State_8_suff_3; State_8_suff_2; State_1_suff_10; State_9_suff_3; State_10_suff_1; State_6_suff_1; State_4_suff_1; State_10; State_3; State_2_suff_0; State_5; State_6; State_9_suff_2; State_1_suff_6; State_3_suff_1; State_2_suff_2; State_1_suff_3; State_4; State_6_suff_2; State_9_suff_6; State_1_suff_5; State_7_suff_1; State_10_suff_0; State_5_suff_3] |}.
+Next Obligation.
+repeat constructor;
+  repeat match goal with
+          | H: List.In _ [] |- _ => apply List.in_nil in H; exfalso; exact H
+          | |- ~ List.In _ [] => apply List.in_nil
+          | |- ~ List.In _ (_ :: _) => unfold not; intros
+          | H: List.In _ (_::_) |- _ => inversion H; clear H
+          | _ => discriminate
+          end.
+Qed.
+Next Obligation.
+  destruct x; intuition congruence.
+Qed.
+Inductive header : nat -> Type :=
+| buf_256: header 256
+| buf_320: header 320
+| buf_192: header 192
+| buf_72: header 72
+| buf_136: header 136
+| buf_200: header 200
+| buf_264: header 264
+| buf_16: header 16
+| buf_80: header 80
+| buf_288: header 288
+| buf_352: header 352
+| buf_32: header 32
+| buf_40: header 40
+| buf_104: header 104
+| buf_168: header 168
+| buf_232: header 232
+| buf_48: header 48.
+Definition h256_eq_dec (x y: header 256) : {x = y} + {x <> y}.
 refine (
   match x with
-  | HdrEth =>
+  | buf_256 =>
     match y with
-    | HdrEth => left eq_refl
+    | buf_256 => left eq_refl
+    end
+  end
+); unfold "<>"; intros H; inversion H.
+Defined.
+Definition h320_eq_dec (x y: header 320) : {x = y} + {x <> y}.
+refine (
+  match x with
+  | buf_320 =>
+    match y with
+    | buf_320 => left eq_refl
+    end
+  end
+); unfold "<>"; intros H; inversion H.
+Defined.
+Definition h192_eq_dec (x y: header 192) : {x = y} + {x <> y}.
+refine (
+  match x with
+  | buf_192 =>
+    match y with
+    | buf_192 => left eq_refl
+    end
+  end
+); unfold "<>"; intros H; inversion H.
+Defined.
+Definition h288_eq_dec (x y: header 288) : {x = y} + {x <> y}.
+refine (
+  match x with
+  | buf_288 =>
+    match y with
+    | buf_288 => left eq_refl
+    end
+  end
+); unfold "<>"; intros H; inversion H.
+Defined.
+Definition h352_eq_dec (x y: header 352) : {x = y} + {x <> y}.
+refine (
+  match x with
+  | buf_352 =>
+    match y with
+    | buf_352 => left eq_refl
     end
   end
 ); unfold "<>"; intros H; inversion H.
@@ -49,93 +381,143 @@ Defined.
 Definition h32_eq_dec (x y: header 32) : {x = y} + {x <> y}.
 refine (
   match x with
-  | HdrICMP =>
+  | buf_32 =>
     match y with
-    | HdrICMP => left eq_refl
-    | HdrICMPv6 => right _
-    end
-  | HdrICMPv6 =>
-    match y with
-    | HdrICMP => right _
-    | HdrICMPv6 => left eq_refl
+    | buf_32 => left eq_refl
     end
   end
 ); unfold "<>"; intros H; inversion H.
 Defined.
-Definition h64_eq_dec (x y: header 64) : {x = y} + {x <> y}.
+Definition h72_eq_dec (x y: header 72) : {x = y} + {x <> y}.
 refine (
   match x with
-  | HdrIPv4 =>
+  | buf_72 =>
     match y with
-    | HdrIPv4 => left eq_refl
-    | HdrIPv6 => right _
-    | HdrARP => right _
-    | HdrARPIP => right _
-    end
-  | HdrIPv6 =>
-    match y with
-    | HdrIPv4 => right _
-    | HdrIPv6 => left eq_refl
-    | HdrARP => right _
-    | HdrARPIP => right _
-    end
-  | HdrARP =>
-    match y with
-    | HdrIPv4 => right _
-    | HdrIPv6 => right _
-    | HdrARP => left eq_refl
-    | HdrARPIP => right _
-    end
-  | HdrARPIP =>
-    match y with
-    | HdrIPv4 => right _
-    | HdrIPv6 => right _
-    | HdrARP => right _
-    | HdrARPIP => left eq_refl
+    | buf_72 => left eq_refl
     end
   end
 ); unfold "<>"; intros H; inversion H.
 Defined.
-Definition h160_eq_dec (x y: header 160) : {x = y} + {x <> y}.
+Definition h136_eq_dec (x y: header 136) : {x = y} + {x <> y}.
 refine (
   match x with
-  | HdrVLAN0 =>
+  | buf_136 =>
     match y with
-    | HdrVLAN0 => left eq_refl
-    | HdrVLAN1 => right _
-    | HdrTCP => right _
-    | HdrUDP => right _
-    end
-  | HdrVLAN1 =>
-    match y with
-    | HdrVLAN0 => right _
-    | HdrVLAN1 => left eq_refl
-    | HdrTCP => right _
-    | HdrUDP => right _
-    end
-  | HdrTCP =>
-    match y with
-    | HdrVLAN0 => right _
-    | HdrVLAN1 => right _
-    | HdrTCP => left eq_refl
-    | HdrUDP => right _
-    end
-  | HdrUDP =>
-    match y with
-    | HdrVLAN0 => right _
-    | HdrVLAN1 => right _
-    | HdrTCP => right _
-    | HdrUDP => left eq_refl
+    | buf_136 => left eq_refl
     end
   end
 ); unfold "<>"; intros H; inversion H.
 Defined.
+Definition h200_eq_dec (x y: header 200) : {x = y} + {x <> y}.
+refine (
+  match x with
+  | buf_200 =>
+    match y with
+    | buf_200 => left eq_refl
+    end
+  end
+); unfold "<>"; intros H; inversion H.
+Defined.
+Definition h264_eq_dec (x y: header 264) : {x = y} + {x <> y}.
+refine (
+  match x with
+  | buf_264 =>
+    match y with
+    | buf_264 => left eq_refl
+    end
+  end
+); unfold "<>"; intros H; inversion H.
+Defined.
+Definition h40_eq_dec (x y: header 40) : {x = y} + {x <> y}.
+refine (
+  match x with
+  | buf_40 =>
+    match y with
+    | buf_40 => left eq_refl
+    end
+  end
+); unfold "<>"; intros H; inversion H.
+Defined.
+Definition h104_eq_dec (x y: header 104) : {x = y} + {x <> y}.
+refine (
+  match x with
+  | buf_104 =>
+    match y with
+    | buf_104 => left eq_refl
+    end
+  end
+); unfold "<>"; intros H; inversion H.
+Defined.
+Definition h168_eq_dec (x y: header 168) : {x = y} + {x <> y}.
+refine (
+  match x with
+  | buf_168 =>
+    match y with
+    | buf_168 => left eq_refl
+    end
+  end
+); unfold "<>"; intros H; inversion H.
+Defined.
+Definition h232_eq_dec (x y: header 232) : {x = y} + {x <> y}.
+refine (
+  match x with
+  | buf_232 =>
+    match y with
+    | buf_232 => left eq_refl
+    end
+  end
+); unfold "<>"; intros H; inversion H.
+Defined.
+Definition h16_eq_dec (x y: header 16) : {x = y} + {x <> y}.
+refine (
+  match x with
+  | buf_16 =>
+    match y with
+    | buf_16 => left eq_refl
+    end
+  end
+); unfold "<>"; intros H; inversion H.
+Defined.
+Definition h80_eq_dec (x y: header 80) : {x = y} + {x <> y}.
+refine (
+  match x with
+  | buf_80 =>
+    match y with
+    | buf_80 => left eq_refl
+    end
+  end
+); unfold "<>"; intros H; inversion H.
+Defined.
+Definition h48_eq_dec (x y: header 48) : {x = y} + {x <> y}.
+refine (
+  match x with
+  | buf_48 =>
+    match y with
+    | buf_48 => left eq_refl
+    end
+  end
+); unfold "<>"; intros H; inversion H.
+Defined.
+Derive Signature for header.
 Definition header_eqdec_ (n: nat) (x: header n) (y: header n) : {x = y} + {x <> y}.
   solve_header_eqdec_ n x y
-    ((existT (fun n => forall x y: header n, {x = y} + {x <> y}) _ h112_eq_dec) ::
+    ((existT (fun n => forall x y: header n, {x = y} + {x <> y}) _ h256_eq_dec) ::
+     (existT _ _ h320_eq_dec) ::
+     (existT _ _ h192_eq_dec) ::
+     (existT _ _ h288_eq_dec) ::
+     (existT _ _ h352_eq_dec) ::
      (existT _ _ h32_eq_dec) ::
-     (existT _ _ h64_eq_dec) ::
-     (existT _ _ h160_eq_dec) ::
+     (existT _ _ h72_eq_dec) ::
+     (existT _ _ h136_eq_dec) ::
+     (existT _ _ h200_eq_dec) ::
+     (existT _ _ h264_eq_dec) ::
+     (existT _ _ h40_eq_dec) ::
+     (existT _ _ h104_eq_dec) ::
+     (existT _ _ h168_eq_dec) ::
+     (existT _ _ h232_eq_dec) ::
+     (existT _ _ h16_eq_dec) ::
+     (existT _ _ h80_eq_dec) ::
+     (existT _ _ h48_eq_dec) ::
       nil).
 Defined.
 
@@ -144,22 +526,28 @@ Global Instance header_eqdec': EquivDec.EqDec (Syntax.H' header) eq.
   solve_eqdec'.
 Defined.
 Global Instance header_finite: forall n, @Finite (header n) _ _.
-  intros n; solve_indexed_finiteness n [112; 32 ; 64 ; 160 ].
+  intros n; solve_indexed_finiteness n [256; 320 ; 192 ; 288 ; 352 ; 32 ; 72 ; 136 ; 200 ; 264 ; 40 ; 104 ; 168 ; 232 ; 16 ; 80 ; 48 ].
 Qed.
 
 Global Program Instance header_finite': @Finite {n & header n} _ header_eqdec' :=
   {| enum := [
-      existT _ _ HdrEth
-    ; existT _ _ HdrVLAN0
-    ; existT _ _ HdrVLAN1
-    ; existT _ _ HdrIPv4
-    ; existT _ _ HdrIPv6
-    ; existT _ _ HdrTCP
-    ; existT _ _ HdrUDP
-    ; existT _ _ HdrICMP
-    ; existT _ _ HdrICMPv6
-    ; existT _ _ HdrARP
-    ; existT _ _ HdrARPIP
+      existT _ _ buf_256
+    ; existT _ _ buf_320
+    ; existT _ _ buf_192
+    ; existT _ _ buf_72
+    ; existT _ _ buf_136
+    ; existT _ _ buf_200
+    ; existT _ _ buf_264
+    ; existT _ _ buf_16
+    ; existT _ _ buf_80
+    ; existT _ _ buf_288
+    ; existT _ _ buf_352
+    ; existT _ _ buf_32
+    ; existT _ _ buf_40
+    ; existT _ _ buf_104
+    ; existT _ _ buf_168
+    ; existT _ _ buf_232
+    ; existT _ _ buf_48
     ] |}.
 Next Obligation.
   solve_header_finite.
@@ -172,118 +560,294 @@ repeat (
   end
 ).
 Qed.
-
-Inductive state: Type :=
-| ParseEth
-| ParseVLAN0
-| ParseVLAN1
-| ParseIPv4
-| ParseIPv6
-| ParseTCP
-| ParseUDP
-| ParseICMP
-| ParseICMPv6
-| ParseARP
-| ParseARPIP.
-
-Scheme Equality for state.
-Global Instance state_eqdec: EquivDec.EqDec state eq := state_eq_dec.
-Global Program Instance state_finite: @Finite state _ state_eq_dec :=
-  {| enum := [ParseEth; ParseVLAN0; ParseVLAN1; ParseIPv4; ParseIPv6; ParseTCP; ParseUDP; ParseICMP; ParseICMPv6; ParseARP; ParseARPIP] |}.
-Next Obligation.
-  repeat constructor;
-    repeat match goal with
-            | H: List.In _ [] |- _ => apply List.in_nil in H; exfalso; exact H
-            | |- ~ List.In _ [] => apply List.in_nil
-            | |- ~ List.In _ (_ :: _) => unfold not; intros
-            | H: List.In _ (_::_) |- _ => inversion H; clear H
-            | _ => discriminate
-            end.
-Qed.
-Next Obligation.
-  destruct x; intuition congruence.
-Qed.
-
-Definition states (s: state) : P4A.state state header :=
+Definition states (s: state) :=
   match s with
-  | ParseEth =>
-    {| st_op := extract(HdrEth);
-       st_trans := transition select (| (EHdr HdrEth)[111--96] |)
-                              {{ [| hexact 0x8100 |] ==> inl ParseVLAN0 ;;;
-                                 [| hexact 0x9100 |] ==> inl ParseVLAN0 ;;;
-                                 [| hexact 0x9200 |] ==> inl ParseVLAN0 ;;;
-                                 [| hexact 0x9300 |] ==> inl ParseVLAN0 ;;;
-                                 [| hexact 0x0800 |] ==> inl ParseIPv4 ;;;
-                                 [| hexact 0x86dd |] ==> inl ParseIPv6 ;;;
-                                 [| hexact 0x0806 |] ==> inl ParseARP ;;;
-                                 [| hexact 0x8035 |] ==> inl ParseARP ;;;
-                                 reject }}
-    |}
-  | ParseVLAN0 =>
-    {| st_op := extract(HdrVLAN0) ;
-       st_trans := transition select (| (EHdr HdrVLAN0)[159--144] |)
-                              {{ [| hexact 0x8100 |] ==> inl ParseVLAN1 ;;;
-                                 [| hexact 0x9100 |] ==> inl ParseVLAN1 ;;;
-                                 [| hexact 0x9200 |] ==> inl ParseVLAN1 ;;;
-                                 [| hexact 0x9300 |] ==> inl ParseVLAN1 ;;;
-                                 [| hexact 0x0800 |] ==> inl ParseIPv4 ;;;
-                                 [| hexact 0x86dd |] ==> inl ParseIPv6 ;;;
-                                 [| hexact 0x0806 |] ==> inl ParseARP ;;;
-                                 [| hexact 0x8035 |] ==> inl ParseARP ;;;
-                                 reject }}
-    |}
-  | ParseVLAN1 =>
-    {| st_op := extract(HdrVLAN1) ;
-       st_trans := transition select (| (EHdr HdrVLAN1)[159--144] |)
-                              {{ [| hexact 0x0800 |] ==> inl ParseIPv4 ;;;
-                                 [| hexact 0x86dd |] ==> inl ParseIPv6 ;;;
-                                 [| hexact 0x0806 |] ==> inl ParseARP ;;;
-                                 [| hexact 0x8035 |] ==> inl ParseARP ;;;
-                                 reject }}
-    |}
-  | ParseIPv4 =>
-    {| st_op := extract(HdrIPv4);
-       st_trans := transition select (| (EHdr HdrIPv4)[79--72] |)
-                              {{ [| hexact 1 |] ==> inl ParseICMP;;;
-                                 [| hexact 6 |] ==> inl ParseTCP;;;
-                                 [| hexact 17 |] ==> inl ParseUDP;;;
-                                 accept
-                              }}
-    |}
-  | ParseIPv6 =>
-    {| st_op := extract(HdrIPv6);
-       st_trans := transition select (| (EHdr HdrIPv6)[55--48] |)
-                              {{ [| hexact 1 |] ==> inl ParseICMPv6;;;
-                                 [| hexact 6 |] ==> inl ParseTCP;;;
-                                 [| hexact 17 |] ==> inl ParseUDP;;;
-                                 accept
-                              }}
-    |}
-  | ParseUDP =>
-    {| st_op := extract(HdrUDP);
-       st_trans := transition accept |}
-  | ParseTCP =>
-    {| st_op := extract(HdrTCP);
-       st_trans := transition accept |}
-  | ParseICMP =>
-    {| st_op := extract(HdrICMP);
-       st_trans := transition accept |}
-  | ParseICMPv6 =>
-    {| st_op := extract(HdrICMPv6);
-       st_trans := transition accept |}
-  | ParseARP =>
-    {| st_op := extract(HdrARP);
-       st_trans := transition select (| (EHdr HdrARP)[31--16] |)
-                              {{ [| hexact 0x0800 |] ==> inl ParseARPIP;;;
-                                 accept
-                              }}
-    |}
-  | ParseARPIP =>
-    {| st_op := extract(HdrARPIP);
-       st_trans := transition accept
-    |}
-  end.
-
+  | State_0 => {|
+    st_op := extract(buf_16);
+    st_trans := transition select (| (EHdr buf_16)[15 -- 15], (EHdr buf_16)[14 -- 14], (EHdr buf_16)[13 -- 13], (EHdr buf_16)[12 -- 12], (EHdr buf_16)[11 -- 11], (EHdr buf_16)[10 -- 10], (EHdr buf_16)[9 -- 9], (EHdr buf_16)[8 -- 8], (EHdr buf_16)[7 -- 7], (EHdr buf_16)[6 -- 6], (EHdr buf_16)[5 -- 5], (EHdr buf_16)[4 -- 4], (EHdr buf_16)[3 -- 3], (EHdr buf_16)[2 -- 2], (EHdr buf_16)[1 -- 1], (EHdr buf_16)[0 -- 0], (EHdr buf_16)[15 -- 15], (EHdr buf_16)[14 -- 14], (EHdr buf_16)[13 -- 13], (EHdr buf_16)[12 -- 12], (EHdr buf_16)[11 -- 11], (EHdr buf_16)[10 -- 10], (EHdr buf_16)[9 -- 9], (EHdr buf_16)[8 -- 8], (EHdr buf_16)[7 -- 7], (EHdr buf_16)[6 -- 6], (EHdr buf_16)[5 -- 5], (EHdr buf_16)[4 -- 4], (EHdr buf_16)[3 -- 3], (EHdr buf_16)[2 -- 2], (EHdr buf_16)[1 -- 1], (EHdr buf_16)[0 -- 0]|) {{
+      [| *, *, *, *, *, *, *, *, *, *, *, *, *, *, *, *, *, *, *, *, *, *, *, *, *, *, *, *, *, *, *, * |] ==> inl State_0_suff_0 ;;;
+      reject
+    }}
+  |}
+  | State_0_suff_0 => {|
+    st_op := extract(buf_80);
+    st_trans := transition inl State_0;
+  |}
+  | State_1 => {|
+    st_op := extract(buf_48);
+    st_trans := transition select (| (EHdr buf_48)[15 -- 15], (EHdr buf_48)[14 -- 14], (EHdr buf_48)[13 -- 13], (EHdr buf_48)[12 -- 12], (EHdr buf_48)[11 -- 11], (EHdr buf_48)[10 -- 10], (EHdr buf_48)[9 -- 9], (EHdr buf_48)[8 -- 8], (EHdr buf_48)[7 -- 7], (EHdr buf_48)[6 -- 6], (EHdr buf_48)[5 -- 5], (EHdr buf_48)[4 -- 4], (EHdr buf_48)[3 -- 3], (EHdr buf_48)[2 -- 2], (EHdr buf_48)[1 -- 1], (EHdr buf_48)[0 -- 0], (EHdr buf_48)[47 -- 47], (EHdr buf_48)[46 -- 46], (EHdr buf_48)[45 -- 45], (EHdr buf_48)[44 -- 44], (EHdr buf_48)[43 -- 43], (EHdr buf_48)[42 -- 42], (EHdr buf_48)[41 -- 41], (EHdr buf_48)[40 -- 40], (EHdr buf_48)[39 -- 39], (EHdr buf_48)[38 -- 38], (EHdr buf_48)[37 -- 37], (EHdr buf_48)[36 -- 36], (EHdr buf_48)[35 -- 35], (EHdr buf_48)[34 -- 34], (EHdr buf_48)[33 -- 33], (EHdr buf_48)[32 -- 32]|) {{
+      [| exact #b|0, exact #b|0, exact #b|0, exact #b|0, exact #b|1, exact #b|0, exact #b|0, exact #b|0, exact #b|0, exact #b|0, exact #b|0, exact #b|0, exact #b|0, exact #b|0, exact #b|0, exact #b|0, *, *, *, *, *, *, *, *, *, *, *, *, *, *, *, * |] ==> reject ;;;
+      [| exact #b|0, exact #b|0, exact #b|0, exact #b|0, exact #b|1, exact #b|0, exact #b|0, exact #b|0, exact #b|0, exact #b|0, exact #b|0, exact #b|0, exact #b|0, exact #b|1, exact #b|1, exact #b|0, *, *, *, *, *, *, *, *, *, *, *, *, *, *, *, * |] ==> reject ;;;
+      [| exact #b|1, exact #b|0, exact #b|0, exact #b|0, exact #b|0, exact #b|0, exact #b|0, exact #b|0, exact #b|0, exact #b|0, exact #b|1, exact #b|1, exact #b|0, exact #b|1, exact #b|0, exact #b|1, *, *, *, *, *, *, *, *, *, *, *, *, *, *, *, * |] ==> reject ;;;
+      [| exact #b|1, exact #b|0, exact #b|0, exact #b|0, exact #b|0, exact #b|1, exact #b|1, exact #b|0, exact #b|1, exact #b|1, exact #b|0, exact #b|1, exact #b|1, exact #b|1, exact #b|0, exact #b|1, *, *, *, *, *, *, *, *, *, *, *, *, *, *, *, * |] ==> inl State_1_suff_3 ;;;
+      [| exact #b|1, exact #b|0, exact #b|0, *, exact #b|0, exact #b|0, exact #b|0, exact #b|1, exact #b|0, exact #b|0, exact #b|0, exact #b|0, exact #b|0, exact #b|0, exact #b|0, exact #b|0, exact #b|0, exact #b|0, exact #b|0, exact #b|0, exact #b|1, exact #b|0, exact #b|0, exact #b|0, exact #b|0, exact #b|0, exact #b|0, exact #b|0, exact #b|0, exact #b|0, exact #b|0, exact #b|0 |] ==> accept ;;;
+      [| exact #b|1, exact #b|0, exact #b|0, *, exact #b|0, exact #b|0, exact #b|0, exact #b|1, exact #b|0, exact #b|0, exact #b|0, exact #b|0, exact #b|0, exact #b|0, exact #b|0, exact #b|0, exact #b|0, exact #b|0, exact #b|0, exact #b|0, exact #b|1, exact #b|0, exact #b|0, exact #b|0, exact #b|0, exact #b|0, exact #b|0, exact #b|0, exact #b|0, exact #b|1, exact #b|1, exact #b|0 |] ==> inl State_1_suff_5 ;;;
+      [| exact #b|1, exact #b|0, exact #b|0, *, exact #b|0, exact #b|0, exact #b|0, exact #b|1, exact #b|0, exact #b|0, exact #b|0, exact #b|0, exact #b|0, exact #b|0, exact #b|0, exact #b|0, exact #b|1, exact #b|0, exact #b|0, exact #b|0, exact #b|0, exact #b|0, exact #b|0, exact #b|0, exact #b|0, exact #b|0, exact #b|1, exact #b|1, exact #b|0, exact #b|1, exact #b|0, exact #b|1 |] ==> inl State_1_suff_6 ;;;
+      [| exact #b|1, exact #b|0, exact #b|0, *, exact #b|0, exact #b|0, exact #b|0, exact #b|1, exact #b|0, exact #b|0, exact #b|0, exact #b|0, exact #b|0, exact #b|0, exact #b|0, exact #b|0, exact #b|1, exact #b|0, exact #b|0, exact #b|0, exact #b|0, exact #b|1, exact #b|1, exact #b|0, exact #b|1, exact #b|1, exact #b|0, exact #b|1, exact #b|1, exact #b|1, exact #b|0, exact #b|1 |] ==> inl State_1_suff_7 ;;;
+      [| exact #b|1, exact #b|0, exact #b|0, *, exact #b|0, exact #b|0, exact #b|0, exact #b|1, exact #b|0, exact #b|0, exact #b|0, exact #b|0, exact #b|0, exact #b|0, exact #b|0, exact #b|0, *, *, *, *, *, *, *, *, *, *, *, *, *, *, *, * |] ==> accept ;;;
+      [| exact #b|1, exact #b|0, exact #b|0, exact #b|1, exact #b|0, exact #b|0, exact #b|1, *, exact #b|0, exact #b|0, exact #b|0, exact #b|0, exact #b|0, exact #b|0, exact #b|0, exact #b|0, exact #b|0, exact #b|0, exact #b|0, exact #b|0, exact #b|1, exact #b|0, exact #b|0, exact #b|0, exact #b|0, exact #b|0, exact #b|0, exact #b|0, exact #b|0, exact #b|0, exact #b|0, exact #b|0 |] ==> accept ;;;
+      [| exact #b|1, exact #b|0, exact #b|0, exact #b|1, exact #b|0, exact #b|0, exact #b|1, *, exact #b|0, exact #b|0, exact #b|0, exact #b|0, exact #b|0, exact #b|0, exact #b|0, exact #b|0, exact #b|0, exact #b|0, exact #b|0, exact #b|0, exact #b|1, exact #b|0, exact #b|0, exact #b|0, exact #b|0, exact #b|0, exact #b|0, exact #b|0, exact #b|0, exact #b|1, exact #b|1, exact #b|0 |] ==> inl State_1_suff_10 ;;;
+      [| exact #b|1, exact #b|0, exact #b|0, exact #b|1, exact #b|0, exact #b|0, exact #b|1, *, exact #b|0, exact #b|0, exact #b|0, exact #b|0, exact #b|0, exact #b|0, exact #b|0, exact #b|0, exact #b|1, exact #b|0, exact #b|0, exact #b|0, exact #b|0, exact #b|0, exact #b|0, exact #b|0, exact #b|0, exact #b|0, exact #b|1, exact #b|1, exact #b|0, exact #b|1, exact #b|0, exact #b|1 |] ==> inl State_1_suff_11 ;;;
+      [| exact #b|1, exact #b|0, exact #b|0, exact #b|1, exact #b|0, exact #b|0, exact #b|1, *, exact #b|0, exact #b|0, exact #b|0, exact #b|0, exact #b|0, exact #b|0, exact #b|0, exact #b|0, exact #b|1, exact #b|0, exact #b|0, exact #b|0, exact #b|0, exact #b|1, exact #b|1, exact #b|0, exact #b|1, exact #b|1, exact #b|0, exact #b|1, exact #b|1, exact #b|1, exact #b|0, exact #b|1 |] ==> inl State_1_suff_12 ;;;
+      [| exact #b|1, exact #b|0, exact #b|0, exact #b|1, exact #b|0, exact #b|0, exact #b|1, *, exact #b|0, exact #b|0, exact #b|0, exact #b|0, exact #b|0, exact #b|0, exact #b|0, exact #b|0, *, *, *, *, *, *, *, *, *, *, *, *, *, *, *, * |] ==> accept ;;;
+      [| *, *, *, *, *, *, *, *, *, *, *, *, *, *, *, *, *, *, *, *, *, *, *, *, *, *, *, *, *, *, *, * |] ==> reject ;;;
+      reject
+    }}
+  |}
+  | State_1_suff_3 => {|
+    st_op := extract(buf_16);
+    st_trans := transition inl State_3;
+  |}
+  | State_1_suff_5 => {|
+    st_op := extract(buf_16);
+    st_trans := transition inl State_5;
+  |}
+  | State_1_suff_6 => {|
+    st_op := extract(buf_16);
+    st_trans := transition inl State_6;
+  |}
+  | State_1_suff_7 => {|
+    st_op := extract(buf_48);
+    st_trans := transition inl State_7;
+  |}
+  | State_1_suff_10 => {|
+    st_op := extract(buf_16);
+    st_trans := transition inl State_10;
+  |}
+  | State_1_suff_11 => {|
+    st_op := extract(buf_16);
+    st_trans := transition inl State_11;
+  |}
+  | State_1_suff_12 => {|
+    st_op := extract(buf_48);
+    st_trans := transition inl State_12;
+  |}
+  | State_2 => {|
+    st_op := extract(buf_16);
+    st_trans := transition select (| (EHdr buf_16)[15 -- 15], (EHdr buf_16)[14 -- 14], (EHdr buf_16)[13 -- 13], (EHdr buf_16)[12 -- 12], (EHdr buf_16)[11 -- 11], (EHdr buf_16)[10 -- 10], (EHdr buf_16)[9 -- 9], (EHdr buf_16)[8 -- 8], (EHdr buf_16)[7 -- 7], (EHdr buf_16)[6 -- 6], (EHdr buf_16)[5 -- 5], (EHdr buf_16)[4 -- 4], (EHdr buf_16)[3 -- 3], (EHdr buf_16)[2 -- 2], (EHdr buf_16)[1 -- 1], (EHdr buf_16)[0 -- 0], (EHdr buf_16)[15 -- 15], (EHdr buf_16)[14 -- 14], (EHdr buf_16)[13 -- 13], (EHdr buf_16)[12 -- 12], (EHdr buf_16)[11 -- 11], (EHdr buf_16)[10 -- 10], (EHdr buf_16)[9 -- 9], (EHdr buf_16)[8 -- 8], (EHdr buf_16)[7 -- 7], (EHdr buf_16)[6 -- 6], (EHdr buf_16)[5 -- 5], (EHdr buf_16)[4 -- 4], (EHdr buf_16)[3 -- 3], (EHdr buf_16)[2 -- 2], (EHdr buf_16)[1 -- 1], (EHdr buf_16)[0 -- 0]|) {{
+      [| exact #b|0, exact #b|0, exact #b|0, exact #b|0, exact #b|0, exact #b|1, exact #b|1, exact #b|0, *, *, *, *, *, *, *, *, *, *, *, *, *, *, *, *, *, *, *, *, *, *, *, * |] ==> inl State_2_suff_0 ;;;
+      [| exact #b|0, exact #b|0, exact #b|0, exact #b|1, exact #b|0, exact #b|0, exact #b|0, exact #b|1, *, *, *, *, *, *, *, *, *, *, *, *, *, *, *, *, *, *, *, *, *, *, *, * |] ==> inl State_2_suff_1 ;;;
+      [| exact #b|0, exact #b|0, exact #b|1, exact #b|1, exact #b|1, exact #b|0, exact #b|1, exact #b|0, *, *, *, *, *, *, *, *, *, *, *, *, *, *, *, *, *, *, *, *, *, *, *, * |] ==> inl State_2_suff_2 ;;;
+      [| *, *, *, *, *, *, *, *, *, *, *, *, *, *, *, *, *, *, *, *, *, *, *, *, *, *, *, *, *, *, *, * |] ==> inl State_2_suff_3 ;;;
+      reject
+    }}
+  |}
+  | State_2_suff_0 => {|
+    st_op := extract(buf_352);
+    st_trans := transition inl State_0;
+  |}
+  | State_2_suff_1 => {|
+    st_op := extract(buf_320);
+    st_trans := transition accept;
+  |}
+  | State_2_suff_2 => {|
+    st_op := extract(buf_288);
+    st_trans := transition accept;
+  |}
+  | State_2_suff_3 => {|
+    st_op := extract(buf_256);
+    st_trans := transition accept;
+  |}
+  | State_3 => {|
+    st_op := extract(buf_16);
+    st_trans := transition select (| (EHdr buf_16)[15 -- 15], (EHdr buf_16)[14 -- 14], (EHdr buf_16)[13 -- 13], (EHdr buf_16)[12 -- 12], (EHdr buf_16)[11 -- 11], (EHdr buf_16)[10 -- 10], (EHdr buf_16)[9 -- 9], (EHdr buf_16)[8 -- 8], (EHdr buf_16)[7 -- 7], (EHdr buf_16)[6 -- 6], (EHdr buf_16)[5 -- 5], (EHdr buf_16)[4 -- 4], (EHdr buf_16)[3 -- 3], (EHdr buf_16)[2 -- 2], (EHdr buf_16)[1 -- 1], (EHdr buf_16)[0 -- 0], (EHdr buf_16)[15 -- 15], (EHdr buf_16)[14 -- 14], (EHdr buf_16)[13 -- 13], (EHdr buf_16)[12 -- 12], (EHdr buf_16)[11 -- 11], (EHdr buf_16)[10 -- 10], (EHdr buf_16)[9 -- 9], (EHdr buf_16)[8 -- 8], (EHdr buf_16)[7 -- 7], (EHdr buf_16)[6 -- 6], (EHdr buf_16)[5 -- 5], (EHdr buf_16)[4 -- 4], (EHdr buf_16)[3 -- 3], (EHdr buf_16)[2 -- 2], (EHdr buf_16)[1 -- 1], (EHdr buf_16)[0 -- 0]|) {{
+      [| exact #b|0, exact #b|1, exact #b|0, exact #b|1, *, *, *, *, *, *, *, *, *, *, *, *, *, *, *, *, *, *, *, *, *, *, *, *, *, *, *, * |] ==> inl State_3_suff_0 ;;;
+      [| exact #b|0, exact #b|1, exact #b|1, exact #b|0, *, *, *, *, *, *, *, *, *, *, *, *, *, *, *, *, *, *, *, *, *, *, *, *, *, *, *, * |] ==> inl State_3_suff_1 ;;;
+      reject
+    }}
+  |}
+  | State_3_suff_0 => {|
+    st_op := extract(buf_48);
+    st_trans := transition accept;
+  |}
+  | State_3_suff_1 => {|
+    st_op := extract(buf_80);
+    st_trans := transition accept;
+  |}
+  | State_4 => {|
+    st_op := extract(buf_40);
+    st_trans := transition select (| (EHdr buf_40)[15 -- 15], (EHdr buf_40)[14 -- 14], (EHdr buf_40)[13 -- 13], (EHdr buf_40)[12 -- 12], (EHdr buf_40)[11 -- 11], (EHdr buf_40)[10 -- 10], (EHdr buf_40)[9 -- 9], (EHdr buf_40)[8 -- 8], (EHdr buf_40)[7 -- 7], (EHdr buf_40)[6 -- 6], (EHdr buf_40)[5 -- 5], (EHdr buf_40)[4 -- 4], (EHdr buf_40)[3 -- 3], (EHdr buf_40)[2 -- 2], (EHdr buf_40)[1 -- 1], (EHdr buf_40)[0 -- 0], (EHdr buf_40)[39 -- 39], (EHdr buf_40)[38 -- 38], (EHdr buf_40)[37 -- 37], (EHdr buf_40)[36 -- 36], (EHdr buf_40)[35 -- 35], (EHdr buf_40)[34 -- 34], (EHdr buf_40)[33 -- 33], (EHdr buf_40)[32 -- 32], (EHdr buf_40)[31 -- 31], (EHdr buf_40)[30 -- 30], (EHdr buf_40)[29 -- 29], (EHdr buf_40)[28 -- 28], (EHdr buf_40)[27 -- 27], (EHdr buf_40)[26 -- 26], (EHdr buf_40)[25 -- 25], (EHdr buf_40)[24 -- 24]|) {{
+      [| *, *, *, exact #b|0, exact #b|0, exact #b|0, exact #b|0, exact #b|0, exact #b|0, exact #b|0, exact #b|0, exact #b|0, exact #b|0, exact #b|0, exact #b|0, exact #b|0, exact #b|0, exact #b|0, exact #b|0, exact #b|0, exact #b|0, exact #b|0, exact #b|0, exact #b|1, *, *, *, *, *, *, *, * |] ==> inl State_4_suff_0 ;;;
+      [| *, *, *, exact #b|0, exact #b|0, exact #b|0, exact #b|0, exact #b|0, exact #b|0, exact #b|0, exact #b|0, exact #b|0, exact #b|0, exact #b|0, exact #b|0, exact #b|0, exact #b|0, exact #b|0, exact #b|0, exact #b|0, exact #b|0, exact #b|1, exact #b|1, exact #b|0, *, *, *, *, *, *, *, * |] ==> inl State_4_suff_1 ;;;
+      [| *, *, *, exact #b|0, exact #b|0, exact #b|0, exact #b|0, exact #b|0, exact #b|0, exact #b|0, exact #b|0, exact #b|0, exact #b|0, exact #b|0, exact #b|0, exact #b|0, exact #b|0, exact #b|0, exact #b|0, exact #b|1, exact #b|0, exact #b|0, exact #b|0, exact #b|1, *, *, *, *, *, *, *, * |] ==> inl State_4_suff_2 ;;;
+      [| *, *, *, *, *, *, *, *, *, *, *, *, *, *, *, *, *, *, *, *, *, *, *, *, *, *, *, *, *, *, *, * |] ==> inl State_4_suff_3 ;;;
+      reject
+    }}
+  |}
+  | State_4_suff_0 => {|
+    st_op := extract(buf_104);
+    st_trans := transition accept;
+  |}
+  | State_4_suff_1 => {|
+    st_op := extract(buf_168);
+    st_trans := transition inl State_1;
+  |}
+  | State_4_suff_2 => {|
+    st_op := extract(buf_136);
+    st_trans := transition accept;
+  |}
+  | State_4_suff_3 => {|
+    st_op := extract(buf_72);
+    st_trans := transition accept;
+  |}
+  | State_5 => {|
+    st_op := extract(buf_40);
+    st_trans := transition select (| (EHdr buf_40)[15 -- 15], (EHdr buf_40)[14 -- 14], (EHdr buf_40)[13 -- 13], (EHdr buf_40)[12 -- 12], (EHdr buf_40)[11 -- 11], (EHdr buf_40)[10 -- 10], (EHdr buf_40)[9 -- 9], (EHdr buf_40)[8 -- 8], (EHdr buf_40)[7 -- 7], (EHdr buf_40)[6 -- 6], (EHdr buf_40)[5 -- 5], (EHdr buf_40)[4 -- 4], (EHdr buf_40)[3 -- 3], (EHdr buf_40)[2 -- 2], (EHdr buf_40)[1 -- 1], (EHdr buf_40)[0 -- 0], (EHdr buf_40)[39 -- 39], (EHdr buf_40)[38 -- 38], (EHdr buf_40)[37 -- 37], (EHdr buf_40)[36 -- 36], (EHdr buf_40)[35 -- 35], (EHdr buf_40)[34 -- 34], (EHdr buf_40)[33 -- 33], (EHdr buf_40)[32 -- 32], (EHdr buf_40)[31 -- 31], (EHdr buf_40)[30 -- 30], (EHdr buf_40)[29 -- 29], (EHdr buf_40)[28 -- 28], (EHdr buf_40)[27 -- 27], (EHdr buf_40)[26 -- 26], (EHdr buf_40)[25 -- 25], (EHdr buf_40)[24 -- 24]|) {{
+      [| *, *, *, exact #b|0, exact #b|0, exact #b|0, exact #b|0, exact #b|0, exact #b|0, exact #b|0, exact #b|0, exact #b|0, exact #b|0, exact #b|0, exact #b|0, exact #b|0, exact #b|0, exact #b|0, exact #b|0, exact #b|0, exact #b|0, exact #b|0, exact #b|0, exact #b|1, *, *, *, *, *, *, *, * |] ==> inl State_5_suff_0 ;;;
+      [| *, *, *, exact #b|0, exact #b|0, exact #b|0, exact #b|0, exact #b|0, exact #b|0, exact #b|0, exact #b|0, exact #b|0, exact #b|0, exact #b|0, exact #b|0, exact #b|0, exact #b|0, exact #b|0, exact #b|0, exact #b|0, exact #b|0, exact #b|1, exact #b|1, exact #b|0, *, *, *, *, *, *, *, * |] ==> inl State_5_suff_1 ;;;
+      [| *, *, *, exact #b|0, exact #b|0, exact #b|0, exact #b|0, exact #b|0, exact #b|0, exact #b|0, exact #b|0, exact #b|0, exact #b|0, exact #b|0, exact #b|0, exact #b|0, exact #b|0, exact #b|0, exact #b|0, exact #b|1, exact #b|0, exact #b|0, exact #b|0, exact #b|1, *, *, *, *, *, *, *, * |] ==> inl State_5_suff_2 ;;;
+      [| *, *, *, *, *, *, *, *, *, *, *, *, *, *, *, *, *, *, *, *, *, *, *, *, *, *, *, *, *, *, *, * |] ==> inl State_5_suff_3 ;;;
+      reject
+    }}
+  |}
+  | State_5_suff_0 => {|
+    st_op := extract(buf_136);
+    st_trans := transition accept;
+  |}
+  | State_5_suff_1 => {|
+    st_op := extract(buf_200);
+    st_trans := transition inl State_1;
+  |}
+  | State_5_suff_2 => {|
+    st_op := extract(buf_168);
+    st_trans := transition accept;
+  |}
+  | State_5_suff_3 => {|
+    st_op := extract(buf_104);
+    st_trans := transition accept;
+  |}
+  | State_6 => {|
+    st_op := extract(buf_40);
+    st_trans := transition select (| (EHdr buf_40)[15 -- 15], (EHdr buf_40)[14 -- 14], (EHdr buf_40)[13 -- 13], (EHdr buf_40)[12 -- 12], (EHdr buf_40)[11 -- 11], (EHdr buf_40)[10 -- 10], (EHdr buf_40)[9 -- 9], (EHdr buf_40)[8 -- 8], (EHdr buf_40)[7 -- 7], (EHdr buf_40)[6 -- 6], (EHdr buf_40)[5 -- 5], (EHdr buf_40)[4 -- 4], (EHdr buf_40)[3 -- 3], (EHdr buf_40)[2 -- 2], (EHdr buf_40)[1 -- 1], (EHdr buf_40)[0 -- 0], (EHdr buf_40)[39 -- 39], (EHdr buf_40)[38 -- 38], (EHdr buf_40)[37 -- 37], (EHdr buf_40)[36 -- 36], (EHdr buf_40)[35 -- 35], (EHdr buf_40)[34 -- 34], (EHdr buf_40)[33 -- 33], (EHdr buf_40)[32 -- 32], (EHdr buf_40)[31 -- 31], (EHdr buf_40)[30 -- 30], (EHdr buf_40)[29 -- 29], (EHdr buf_40)[28 -- 28], (EHdr buf_40)[27 -- 27], (EHdr buf_40)[26 -- 26], (EHdr buf_40)[25 -- 25], (EHdr buf_40)[24 -- 24]|) {{
+      [| *, *, *, exact #b|0, exact #b|0, exact #b|0, exact #b|0, exact #b|0, exact #b|0, exact #b|0, exact #b|0, exact #b|0, exact #b|0, exact #b|0, exact #b|0, exact #b|0, exact #b|0, exact #b|0, exact #b|0, exact #b|0, exact #b|0, exact #b|0, exact #b|0, exact #b|1, *, *, *, *, *, *, *, * |] ==> inl State_6_suff_0 ;;;
+      [| *, *, *, exact #b|0, exact #b|0, exact #b|0, exact #b|0, exact #b|0, exact #b|0, exact #b|0, exact #b|0, exact #b|0, exact #b|0, exact #b|0, exact #b|0, exact #b|0, exact #b|0, exact #b|0, exact #b|0, exact #b|0, exact #b|0, exact #b|1, exact #b|1, exact #b|0, *, *, *, *, *, *, *, * |] ==> inl State_6_suff_1 ;;;
+      [| *, *, *, exact #b|0, exact #b|0, exact #b|0, exact #b|0, exact #b|0, exact #b|0, exact #b|0, exact #b|0, exact #b|0, exact #b|0, exact #b|0, exact #b|0, exact #b|0, exact #b|0, exact #b|0, exact #b|0, exact #b|1, exact #b|0, exact #b|0, exact #b|0, exact #b|1, *, *, *, *, *, *, *, * |] ==> inl State_6_suff_2 ;;;
+      [| *, *, *, *, *, *, *, *, *, *, *, *, *, *, *, *, *, *, *, *, *, *, *, *, *, *, *, *, *, *, *, * |] ==> inl State_6_suff_3 ;;;
+      reject
+    }}
+  |}
+  | State_6_suff_0 => {|
+    st_op := extract(buf_168);
+    st_trans := transition accept;
+  |}
+  | State_6_suff_1 => {|
+    st_op := extract(buf_232);
+    st_trans := transition inl State_1;
+  |}
+  | State_6_suff_2 => {|
+    st_op := extract(buf_200);
+    st_trans := transition accept;
+  |}
+  | State_6_suff_3 => {|
+    st_op := extract(buf_136);
+    st_trans := transition accept;
+  |}
+  | State_7 => {|
+    st_op := extract(buf_40);
+    st_trans := transition select (| (EHdr buf_40)[15 -- 15], (EHdr buf_40)[14 -- 14], (EHdr buf_40)[13 -- 13], (EHdr buf_40)[12 -- 12], (EHdr buf_40)[11 -- 11], (EHdr buf_40)[10 -- 10], (EHdr buf_40)[9 -- 9], (EHdr buf_40)[8 -- 8], (EHdr buf_40)[7 -- 7], (EHdr buf_40)[6 -- 6], (EHdr buf_40)[5 -- 5], (EHdr buf_40)[4 -- 4], (EHdr buf_40)[3 -- 3], (EHdr buf_40)[2 -- 2], (EHdr buf_40)[1 -- 1], (EHdr buf_40)[0 -- 0], (EHdr buf_40)[39 -- 39], (EHdr buf_40)[38 -- 38], (EHdr buf_40)[37 -- 37], (EHdr buf_40)[36 -- 36], (EHdr buf_40)[35 -- 35], (EHdr buf_40)[34 -- 34], (EHdr buf_40)[33 -- 33], (EHdr buf_40)[32 -- 32], (EHdr buf_40)[31 -- 31], (EHdr buf_40)[30 -- 30], (EHdr buf_40)[29 -- 29], (EHdr buf_40)[28 -- 28], (EHdr buf_40)[27 -- 27], (EHdr buf_40)[26 -- 26], (EHdr buf_40)[25 -- 25], (EHdr buf_40)[24 -- 24]|) {{
+      [| *, *, *, exact #b|0, exact #b|0, exact #b|0, exact #b|0, exact #b|0, exact #b|0, exact #b|0, exact #b|0, exact #b|0, exact #b|0, exact #b|0, exact #b|0, exact #b|0, exact #b|0, exact #b|0, exact #b|0, exact #b|0, exact #b|0, exact #b|0, exact #b|0, exact #b|1, *, *, *, *, *, *, *, * |] ==> inl State_7_suff_0 ;;;
+      [| *, *, *, exact #b|0, exact #b|0, exact #b|0, exact #b|0, exact #b|0, exact #b|0, exact #b|0, exact #b|0, exact #b|0, exact #b|0, exact #b|0, exact #b|0, exact #b|0, exact #b|0, exact #b|0, exact #b|0, exact #b|0, exact #b|0, exact #b|1, exact #b|1, exact #b|0, *, *, *, *, *, *, *, * |] ==> inl State_7_suff_1 ;;;
+      [| *, *, *, exact #b|0, exact #b|0, exact #b|0, exact #b|0, exact #b|0, exact #b|0, exact #b|0, exact #b|0, exact #b|0, exact #b|0, exact #b|0, exact #b|0, exact #b|0, exact #b|0, exact #b|0, exact #b|0, exact #b|1, exact #b|0, exact #b|0, exact #b|0, exact #b|1, *, *, *, *, *, *, *, * |] ==> inl State_7_suff_2 ;;;
+      [| *, *, *, *, *, *, *, *, *, *, *, *, *, *, *, *, *, *, *, *, *, *, *, *, *, *, *, *, *, *, *, * |] ==> inl State_7_suff_3 ;;;
+      reject
+    }}
+  |}
+  | State_7_suff_0 => {|
+    st_op := extract(buf_200);
+    st_trans := transition accept;
+  |}
+  | State_7_suff_1 => {|
+    st_op := extract(buf_264);
+    st_trans := transition inl State_1;
+  |}
+  | State_7_suff_2 => {|
+    st_op := extract(buf_232);
+    st_trans := transition accept;
+  |}
+  | State_7_suff_3 => {|
+    st_op := extract(buf_168);
+    st_trans := transition accept;
+  |}
+  | State_8 => {|
+    st_op := extract(buf_16);
+    st_trans := transition select (| (EHdr buf_16)[15 -- 15], (EHdr buf_16)[14 -- 14], (EHdr buf_16)[13 -- 13], (EHdr buf_16)[12 -- 12], (EHdr buf_16)[11 -- 11], (EHdr buf_16)[10 -- 10], (EHdr buf_16)[9 -- 9], (EHdr buf_16)[8 -- 8], (EHdr buf_16)[7 -- 7], (EHdr buf_16)[6 -- 6], (EHdr buf_16)[5 -- 5], (EHdr buf_16)[4 -- 4], (EHdr buf_16)[3 -- 3], (EHdr buf_16)[2 -- 2], (EHdr buf_16)[1 -- 1], (EHdr buf_16)[0 -- 0], (EHdr buf_16)[15 -- 15], (EHdr buf_16)[14 -- 14], (EHdr buf_16)[13 -- 13], (EHdr buf_16)[12 -- 12], (EHdr buf_16)[11 -- 11], (EHdr buf_16)[10 -- 10], (EHdr buf_16)[9 -- 9], (EHdr buf_16)[8 -- 8], (EHdr buf_16)[7 -- 7], (EHdr buf_16)[6 -- 6], (EHdr buf_16)[5 -- 5], (EHdr buf_16)[4 -- 4], (EHdr buf_16)[3 -- 3], (EHdr buf_16)[2 -- 2], (EHdr buf_16)[1 -- 1], (EHdr buf_16)[0 -- 0]|) {{
+      [| *, *, *, *, exact #b|0, exact #b|1, exact #b|0, exact #b|1, *, *, *, *, *, *, *, *, *, *, *, *, *, *, *, *, *, *, *, *, *, *, *, * |] ==> inl State_8_suff_0 ;;;
+      [| *, *, *, *, exact #b|0, exact #b|1, exact #b|1, exact #b|0, *, *, *, *, *, *, *, *, *, *, *, *, *, *, *, *, *, *, *, *, *, *, *, * |] ==> inl State_8_suff_1 ;;;
+      [| *, *, *, *, exact #b|0, exact #b|1, exact #b|1, exact #b|1, *, *, *, *, *, *, *, *, *, *, *, *, *, *, *, *, *, *, *, *, *, *, *, * |] ==> inl State_8_suff_2 ;;;
+      [| *, *, *, *, exact #b|1, exact #b|0, exact #b|0, exact #b|0, *, *, *, *, *, *, *, *, *, *, *, *, *, *, *, *, *, *, *, *, *, *, *, * |] ==> inl State_8_suff_3 ;;;
+      reject
+    }}
+  |}
+  | State_8_suff_0 => {|
+    st_op := extract(buf_32);
+    st_trans := transition inl State_0;
+  |}
+  | State_8_suff_1 => {|
+    st_op := extract(buf_32);
+    st_trans := transition inl State_1;
+  |}
+  | State_8_suff_2 => {|
+    st_op := extract(buf_32);
+    st_trans := transition inl State_2;
+  |}
+  | State_8_suff_3 => {|
+    st_op := extract(buf_32);
+    st_trans := transition inl State_3;
+  |}
+  | State_9 => {|
+    st_op := extract(buf_32);
+    st_trans := transition select (| (EHdr buf_32)[15 -- 15], (EHdr buf_32)[14 -- 14], (EHdr buf_32)[13 -- 13], (EHdr buf_32)[12 -- 12], (EHdr buf_32)[11 -- 11], (EHdr buf_32)[10 -- 10], (EHdr buf_32)[9 -- 9], (EHdr buf_32)[8 -- 8], (EHdr buf_32)[7 -- 7], (EHdr buf_32)[6 -- 6], (EHdr buf_32)[5 -- 5], (EHdr buf_32)[4 -- 4], (EHdr buf_32)[3 -- 3], (EHdr buf_32)[2 -- 2], (EHdr buf_32)[1 -- 1], (EHdr buf_32)[0 -- 0], (EHdr buf_32)[31 -- 31], (EHdr buf_32)[30 -- 30], (EHdr buf_32)[29 -- 29], (EHdr buf_32)[28 -- 28], (EHdr buf_32)[27 -- 27], (EHdr buf_32)[26 -- 26], (EHdr buf_32)[25 -- 25], (EHdr buf_32)[24 -- 24], (EHdr buf_32)[23 -- 23], (EHdr buf_32)[22 -- 22], (EHdr buf_32)[21 -- 21], (EHdr buf_32)[20 -- 20], (EHdr buf_32)[19 -- 19], (EHdr buf_32)[18 -- 18], (EHdr buf_32)[17 -- 17], (EHdr buf_32)[16 -- 16]|) {{
+      [| exact #b|0, exact #b|0, exact #b|0, exact #b|0, exact #b|1, exact #b|0, exact #b|0, exact #b|0, exact #b|0, exact #b|0, exact #b|0, exact #b|0, exact #b|0, exact #b|0, exact #b|0, exact #b|0, *, *, *, *, exact #b|0, exact #b|1, exact #b|0, exact #b|1, *, *, *, *, *, *, *, * |] ==> inl State_9_suff_0 ;;;
+      [| exact #b|0, exact #b|0, exact #b|0, exact #b|0, exact #b|1, exact #b|0, exact #b|0, exact #b|0, exact #b|0, exact #b|0, exact #b|0, exact #b|0, exact #b|0, exact #b|0, exact #b|0, exact #b|0, *, *, *, *, exact #b|0, exact #b|1, exact #b|1, exact #b|0, *, *, *, *, *, *, *, * |] ==> inl State_9_suff_1 ;;;
+      [| exact #b|0, exact #b|0, exact #b|0, exact #b|0, exact #b|1, exact #b|0, exact #b|0, exact #b|0, exact #b|0, exact #b|0, exact #b|0, exact #b|0, exact #b|0, exact #b|0, exact #b|0, exact #b|0, *, *, *, *, exact #b|0, exact #b|1, exact #b|1, exact #b|1, *, *, *, *, *, *, *, * |] ==> inl State_9_suff_2 ;;;
+      [| exact #b|0, exact #b|0, exact #b|0, exact #b|0, exact #b|1, exact #b|0, exact #b|0, exact #b|0, exact #b|0, exact #b|0, exact #b|0, exact #b|0, exact #b|0, exact #b|0, exact #b|0, exact #b|0, *, *, *, *, exact #b|1, exact #b|0, exact #b|0, exact #b|0, *, *, *, *, *, *, *, * |] ==> inl State_9_suff_3 ;;;
+      [| exact #b|0, exact #b|0, exact #b|0, exact #b|0, exact #b|1, exact #b|0, exact #b|0, exact #b|0, exact #b|0, exact #b|0, exact #b|0, exact #b|0, exact #b|0, exact #b|1, exact #b|1, exact #b|0, *, *, *, *, *, *, *, *, *, *, *, *, *, *, *, * |] ==> accept ;;;
+      [| exact #b|1, exact #b|0, exact #b|0, exact #b|0, exact #b|0, exact #b|0, exact #b|0, exact #b|0, exact #b|0, exact #b|0, exact #b|1, exact #b|1, exact #b|0, exact #b|1, exact #b|0, exact #b|1, *, *, *, *, *, *, *, *, *, *, *, *, *, *, *, * |] ==> accept ;;;
+      [| exact #b|1, exact #b|0, exact #b|0, exact #b|0, exact #b|0, exact #b|1, exact #b|1, exact #b|0, exact #b|1, exact #b|1, exact #b|0, exact #b|1, exact #b|1, exact #b|1, exact #b|0, exact #b|1, *, *, *, *, *, *, *, *, *, *, *, *, *, *, *, * |] ==> inl State_9_suff_6 ;;;
+      [| exact #b|1, exact #b|0, exact #b|0, *, exact #b|0, exact #b|0, exact #b|0, exact #b|1, exact #b|0, exact #b|0, exact #b|0, exact #b|0, exact #b|0, exact #b|0, exact #b|0, exact #b|0, *, *, *, *, *, *, *, *, *, *, *, *, *, *, *, * |] ==> accept ;;;
+      [| exact #b|1, exact #b|0, exact #b|0, exact #b|1, exact #b|0, exact #b|0, exact #b|1, *, exact #b|0, exact #b|0, exact #b|0, exact #b|0, exact #b|0, exact #b|0, exact #b|0, exact #b|0, *, *, *, *, *, *, *, *, *, *, *, *, *, *, *, * |] ==> accept ;;;
+      [| *, *, *, *, *, *, *, *, *, *, *, *, *, *, *, *, *, *, *, *, *, *, *, *, *, *, *, *, *, *, *, * |] ==> reject ;;;
+      reject
+    }}
+  |}
+  | State_9_suff_0 => {|
+    st_op := extract(buf_32);
+    st_trans := transition inl State_0;
+  |}
+  | State_9_suff_1 => {|
+    st_op := extract(buf_32);
+    st_trans := transition inl State_1;
+  |}
+  | State_9_suff_2 => {|
+    st_op := extract(buf_32);
+    st_trans := transition inl State_2;
+  |}
+  | State_9_suff_3 => {|
+    st_op := extract(buf_32);
+    st_trans := transition inl State_3;
+  |}
+  | State_9_suff_6 => {|
+    st_op := extract(buf_32);
+    st_trans := transition inl State_6;
+  |}
+  | State_10 => {|
+    st_op := extract(buf_16);
+    st_trans := transition select (| (EHdr buf_16)[15 -- 15], (EHdr buf_16)[14 -- 14], (EHdr buf_16)[13 -- 13], (EHdr buf_16)[12 -- 12], (EHdr buf_16)[11 -- 11], (EHdr buf_16)[10 -- 10], (EHdr buf_16)[9 -- 9], (EHdr buf_16)[8 -- 8], (EHdr buf_16)[7 -- 7], (EHdr buf_16)[6 -- 6], (EHdr buf_16)[5 -- 5], (EHdr buf_16)[4 -- 4], (EHdr buf_16)[3 -- 3], (EHdr buf_16)[2 -- 2], (EHdr buf_16)[1 -- 1], (EHdr buf_16)[0 -- 0], (EHdr buf_16)[15 -- 15], (EHdr buf_16)[14 -- 14], (EHdr buf_16)[13 -- 13], (EHdr buf_16)[12 -- 12], (EHdr buf_16)[11 -- 11], (EHdr buf_16)[10 -- 10], (EHdr buf_16)[9 -- 9], (EHdr buf_16)[8 -- 8], (EHdr buf_16)[7 -- 7], (EHdr buf_16)[6 -- 6], (EHdr buf_16)[5 -- 5], (EHdr buf_16)[4 -- 4], (EHdr buf_16)[3 -- 3], (EHdr buf_16)[2 -- 2], (EHdr buf_16)[1 -- 1], (EHdr buf_16)[0 -- 0]|) {{
+      [| exact #b|0, exact #b|0, exact #b|0, exact #b|0, exact #b|1, exact #b|0, exact #b|0, exact #b|0, exact #b|0, exact #b|0, exact #b|0, exact #b|0, exact #b|0, exact #b|0, exact #b|0, exact #b|0, *, *, *, *, *, *, *, *, *, *, *, *, *, *, *, * |] ==> inl State_10_suff_0 ;;;
+      [| *, *, *, *, *, *, *, *, *, *, *, *, *, *, *, *, *, *, *, *, *, *, *, *, *, *, *, *, *, *, *, * |] ==> inl State_10_suff_1 ;;;
+      reject
+    }}
+  |}
+  | State_10_suff_0 => {|
+    st_op := extract(buf_192);
+    st_trans := transition accept;
+  |}
+  | State_10_suff_1 => {|
+    st_op := extract(buf_32);
+    st_trans := transition accept;
+  |}
+end.
 Program Definition aut: Syntax.t state header :=
   {| t_states := states |}.
 Solve Obligations with (destruct s; cbv; Lia.lia).
+End Optimized. *)
